src/program_proof/memkv/print_assumptions.v
@@ -1,8 +1,8 @@
 From Perennial.program_proof Require Import proof_prelude.
 From Perennial.program_proof.memkv Require Import closed memkv_clerk_proof.
 
-(* Closed proof for shard server *)
-Print Assumptions shard_boot1.
+(* Closed proof for shard + coord server *)
+Print Assumptions shard_coord_boot.
 
 (* Client proofs -- not yet closed *)
 Definition client_theorems := (@KVClerk__Get, @KVClerk__Put, @KVClerk__ConditionalPut).
